rewrite implementation of exp

code/experimental/rsa/Exponentiation.fst
@@ -13,31 +13,24 @@ module U32 = FStar.UInt32
 module U64 = FStar.UInt64
 module Div = Division
 
-type exp_state (rLen:bnlen) (aLen:bnlen) = lbignum U32.(rLen +^ aLen +^ (aLen +^ aLen) +^ (rLen +^ aLen))
+type exp_state (rLen:bnlen) (aLen:bnlen) = lbignum U32.(rLen +^ (rLen +^ rLen) +^ (rLen +^ aLen))
 
-let get_acc #r #a (st:exp_state r a) : lbignum r = Buffer.sub st 0ul r
-let get_a_1 #r #a (st:exp_state r a) : lbignum a = Buffer.sub st r a
-let get_a2 #r #a (st:exp_state r a) : lbignum U32.(a +^ a) = Buffer.sub st U32.(r +^ a) U32.(a +^ a)
-let get_acc2 #r #a (st:exp_state r a) :lbignum U32.(a +^ r) = Buffer.sub st U32.(r +^ a +^ (a +^ a)) U32.(r +^ a)
+let get_res #r #a (st:exp_state r a) : lbignum r = Buffer.sub st 0ul r
+let get_acc2 #r #a (st:exp_state r a) :lbignum U32.(r +^ r) = Buffer.sub st r U32.(r +^ r)
+let get_a2 #r #a (st:exp_state r a) : lbignum U32.(r +^ a) = Buffer.sub st U32.(r +^ (r +^ r)) U32.(r +^ a)
 
 let exp_state_inv r a (st:exp_state r a) = 
-           let acc = get_acc st in
-           let a = get_a_1 st in
+           let res = get_res st in
            let a2 = get_a2 st in
            let acc2 = get_acc2 st in
-           let r = frameOf acc in
-	     r == frameOf a /\
+           let r = frameOf res in
 	     r == frameOf a2 /\
 	     r == frameOf acc2 /\
-	     disjoint acc a /\
-	     disjoint acc a2 /\
-	     disjoint acc acc2 /\ 
-	     disjoint a a2 /\ 
-	     disjoint a acc2 /\ 
+	     disjoint res a2 /\
+	     disjoint res acc2 /\
        	 disjoint acc2 a2 
 
-
-let exp_state_st_inv (rLen:bnlen) (aLen:bnlen) (st:exp_state rLen aLen) (h:FStar.HyperStack.mem) = 
+let exp_state_st_inv (rLen:bnlen) (aLen:bnlen) (st:exp_state rLen aLen) (h:FStar.HyperStack.mem) =
 	     exp_state_inv rLen aLen st /\ live h st
 
 (* check if input[ind] is equal to 1 *)
@@ -55,62 +48,50 @@ let bn_bit_is_set input ind =
     let res = U64.(((tmp >>^ j) &^ 1uL) =^ 1uL) in
     res
 
-val mod_exp_loop_:
+#reset-options "--z3rlimit 150 --max_fuel 0"
+
+val mod_exp_:
     modBits:U32.t{U32.v modBits > 0} -> aLen:bnlen ->
     bBits:U32.t{U32.v bBits > 0} -> resLen:bnlen ->
     n:lbignum (bits_to_bn modBits) ->
+    a:lbignum aLen ->
     b:lbignum (bits_to_bn bBits) ->
-    st:exp_state resLen aLen{disjoint st n /\ disjoint st b} ->
-    count:U32.t{U32.v count <= U32.v bBits} -> Stack unit
-    (requires (fun h -> live h n /\ live h b /\ exp_state_st_inv resLen aLen st h))
-    (ensures  (fun h0 _ h1 -> live h1 n /\ live h1 b /\ exp_state_st_inv resLen aLen st h1 /\
+    st:exp_state resLen aLen{disjoint st n /\ disjoint st b /\ disjoint st a} ->
+    count:U32.t{U32.v count <= U32.v bBits} ->
+    Stack unit
+    (requires (fun h -> live h n /\ live h b /\ live h a /\ exp_state_st_inv resLen aLen st h))
+    (ensures  (fun h0 _ h1 -> live h0 n /\ live h0 b /\ live h0 a /\ exp_state_st_inv resLen aLen st h0 /\
+                live h1 n /\ live h1 b /\ live h1 a /\ exp_state_st_inv resLen aLen st h1 /\
                 modifies_1 st h0 h1))
 
-#set-options "--z3rlimit 150"
+#reset-options "--z3rlimit 150 --max_fuel 2"
 
-let mod_exp_loop_ modBits aLen bBits resLen n b st count =
-    let acc = get_acc st in
-    let a = get_a_1 st in
-    let acc2 = get_acc2 st in
-    let acc2Len = U32.(resLen +^ aLen) in
-    fill acc2 0uL acc2Len;
+let rec mod_exp_ modBits aLen bBits resLen n a b st count =
+    let a2Len = U32.(resLen +^ aLen) in
+    let acc2Len = U32.(resLen +^ resLen) in
 
-    let diffBits2 = U32.(64ul *^ acc2Len -%^ modBits) in
+    let res : lbignum resLen = get_res st in
+    let a2 : lbignum a2Len = get_a2 st in
+    let acc2 : lbignum acc2Len = get_acc2 st in
+
+    let diffBits1 = U32.(64ul *^ acc2Len -%^ modBits) in
+    let diffBits2 = U32.(64ul *^ a2Len -%^ modBits) in
     let modLen = bits_to_bn modBits in
 
-    (if (bn_bit_is_set b count) then begin
-        mult resLen acc aLen a acc2;
-        Div.remainder acc2Len modLen resLen diffBits2 acc2 n acc
-    end)
+    if U32.(count <^ bBits) then begin
+        mod_exp_ modBits aLen bBits resLen n a b st U32.(count +^ 1ul); //st <- res; acc2; a2
+        
+        fill acc2 0uL acc2Len;
+        sqr resLen res acc2; //acc2 = res * res
+        assume(U32.v modLen <= U32.v acc2Len);
+        Div.remainder acc2Len modLen resLen diffBits1 acc2 n res; // res = acc2 % n
 
-(* mod_exp_loop modBits aLen bBits resLen n a1 b acc count *)
-val mod_exp_loop:
-    modBits:U32.t{U32.v modBits > 0} -> aLen:bnlen ->
-    bBits:U32.t{U32.v bBits > 0} -> resLen:bnlen ->
-    n:lbignum (bits_to_bn modBits) ->
-    b:lbignum (bits_to_bn bBits) ->
-    st:exp_state resLen aLen{disjoint st n /\ disjoint st b} ->
-    count:U32.t{U32.v count <= U32.v bBits} -> Stack unit
-    (requires (fun h -> live h n /\ live h b /\ exp_state_st_inv resLen aLen st h))
-    (ensures  (fun h0 _ h1 -> live h1 n /\ live h1 b /\ exp_state_st_inv resLen aLen st h1 /\
-                modifies_1 st h0 h1))
-
-#set-options "--z3rlimit 150 --max_fuel 2"
-
-let rec mod_exp_loop modBits aLen bBits resLen n b st count =
-    let a = get_a_1 st in
-    let a2 = get_a2 st in
-    let a2Len = U32.(aLen +^ aLen) in
-    fill a2 0uL a2Len;
-
-    let diffBits1 = U32.(64ul *^ a2Len -%^ modBits) in
-    let modLen = bits_to_bn modBits in
-    (if U32.(count <^ bBits) then begin
-        sqr aLen a a2;
-        Div.remainder a2Len modLen aLen diffBits1 a2 n a;
-        mod_exp_loop_ modBits aLen bBits resLen n b st count;
-        mod_exp_loop modBits aLen bBits resLen n b st U32.(count +^ 1ul)
-    end)
+        (if (bn_bit_is_set b count) then begin
+            fill a2 0uL a2Len;
+            mult resLen res aLen a a2; //a2 = res * a
+            assume(U32.v modLen <= U32.v a2Len);
+            Div.remainder a2Len modLen resLen diffBits2 a2 n res end) //res = a2 % n
+    end
 
 (* res = a ^^ b mod n *)
 val mod_exp:
@@ -129,15 +110,9 @@ val mod_exp:
 
 let mod_exp modBits aLen bBits resLen n a b res =
     push_frame();
-    let st : exp_state resLen aLen = create 0uL U32.(resLen +^ aLen +^ (aLen +^ aLen) +^ (resLen +^ aLen)) in
-    let acc = get_acc st in
-    let a_1 = get_a_1 st in
-    blit a 0ul a_1 0ul aLen;
-
-    (if (bn_bit_is_set b 0ul) then
-        blit a_1 0ul acc 0ul aLen
-    else acc.(0ul) <- 1uL);
-
-    mod_exp_loop modBits aLen bBits resLen n b st 1ul;
-    blit acc 0ul res 0ul resLen;
+    let st : exp_state resLen aLen = create 0uL U32.(resLen +^ (resLen +^ resLen) +^ (resLen +^ aLen)) in
+    let res' = get_res st in
+    res'.(0ul) <- 1uL;
+    mod_exp_ modBits aLen bBits resLen n a b st 0ul;
+    blit res' 0ul res 0ul resLen;
     pop_frame()
